Add: opposite'_opposite

theories/D.v
@@ -107,6 +107,44 @@ Defined.
 
 Definition opposite (A B : Type) : Type := prod (contradict A B) (sum A B) .
 
-Definition unique (A B : Type) : Type := is_contr (sum A B) .
+Definition opposite' (A B : Type) : Type := is_contr (sum A B) .
 
-(* todo: opposite A B <-> unique A B *)
+Definition opposite'_opposite
+  {A B : Type} (H : opposite' A B) : opposite A B .
+Proof.
+ unfold opposite .
+ unfold opposite' in H .
+ unfold is_contr in H .
+ refine (dsum_elim_nodep _ H) .
+ refine (fun Hv HH => _) .
+ refine (pair _ _) .
+ -
+  unfold contradict .
+  refine (fun a b => _) .
+  revert Hv HH .
+  refine (sum_elim _ _) .
+  +
+   refine (fun Hva I => _) .
+   refine (cast (A := unit) (B := empty) _ tt) .
+   pose (
+     D
+       := sum_elim_nodep (const unit) (const empty)
+       : sum A B -> Type ) .
+   change (paths (D (left Hva)) (D (right b))) .
+   refine (ap D _) .
+   unfold is_contr_center in I .
+   exact (I (right b)) .
+  +
+   refine (fun Hvb I => _) .
+   refine (cast (A := unit) (B := empty) _ tt) .
+   pose (
+     D
+       := sum_elim_nodep (const empty) (const unit)
+       : sum A B -> Type ) .
+   change (paths (D (right Hvb)) (D (left a))) .
+   refine (ap D _) .
+   unfold is_contr_center in I .
+   exact (I (left a)) .
+ -
+  exact Hv .
+Defined.
